GraphQL.lean
@@ -1,7 +1,6 @@
 import GraphQL.Schema
 import GraphQL.SchemaWellFormedness
 import GraphQL.Operation
-import GraphQL.Semantic
 import GraphQL.FieldMerge
 import GraphQL.Validation
 import GraphQL.NormalForm
